### Test Yourself

1. An integer is even if, and only if, **it equals twice some integer.**

2. An integer is odd if, and only if, **it equals twice some integer plus 1**

3. An integer n is prime if **n is greater than 1 **, and only if,**the only positive factors of n are 1 and n **.

4. The most common way to disprove a universal statement is to find **a counterexample**.

### Exercise Set 4.1

1. a. yes, b.yes, c.yes

2. a. yes,

   b. yes, 

   c. no. $(m-n)(m+n)$, when $m-n = 1$ and $m+n$ is prime, $m^2 - n^2$ is not composite.

3. a. yes. $2(2rs)$ is even, 

   b. yes, $2(3r + 2s^2 + 1)+1$ 

   c. yes, $(r+s)^2$. has a divisor $(r+s)$ at least 2 and won't be itself.

4. exists. $\frac{1}2 + \frac{1}2 = 1$

5. $\frac{1}{-3} + \frac{1}3 = 0$

6. a = 0 or b = 0.

7. $n = 2k$, $2^{2k} - 1 = (2^k + 1)(2^k - 1)$ is composite. $n = 7, 2^n - 1 = 127$.

8. There exists a real number x such that $x > 1$ and $2^x > x^{10}$
     $$2^{1.05} \approx 2.07053$$
     $$1.05^{10} \approx 1.62889$$
     $$1.0776^{10} \approx 2^{1.0776} \approx 2.1104$$
     When $x > 1.0776$ then $2^x < x^{10}$

9. There is a perfect square that can be written as a sum of two other perfect squares.

     $c^2 = a^2 + b^2 = (a + b)^2 - 2ab$ 

     Right triangle: $5^2 = 4^2 + 3^2$

10. $2n^2 - 5n + 2 = (2n -1)(n - 2)$ is prime when ~~n = 1~~(prime is only defined for positive integer) or n = 3.

11. $-3 < 2, (-3)^2 > 2^2$

12. n is odd. $\frac{n-1}{2} = 2k, n = 4k + 1$

13. $2m + n = 2k + 1, \frac{n-1}2 = k - m$, n has to be odd and there is no requirement for m.

$$m = 10, n = 7,2m + n = 27$$

14. $(a + b)^2 = a^2 + b^2$ is true when a = 0 or b = 0.

15. $-a^n = (-a)^n$ true if n is odd, false if n is even

16. $\frac{2a + 1 + 2b + 1}2 = a + b + 1$. true for some, while false for others.

17. Every positive even integer less than 26 can be expressed as a sum of three or fewer perfect squares. (For instance, $10 = 1^2 + 3^2$ and $16 = 4^2$.)


|   2   |1 + 1     |
| ----- | -------- |
|   4   |4 + 0     |
|   6   |4 + 1 + 1 |
|   8   |4 + 4     |
|   10  |9 + 1     |
|   12  |4 + 4 + 4 |
|   14  |9 + 4 + 1 |
|   16  |16        |
|   18  |16 + 1 + 1|
|       |9 + 9     |
|   20  |16 + 4    |
|   22  |9 + 9 + 4 |
|   24  |16 + 4 + 4|

18. For each integer n with $1 \leq n \leq 10, n^2 - n + 11$ is a prime number.

|  1  |$$1^2 - 1 + 11$$| 11 |
| --- | -------------- | -- |
|  2  |$$2^2 - 2 + 11$$| 13 |
|  3  |$$3^2 - 3 + 11$$| 17 |
|  4  |$$4^2 - 4 + 11$$| 23 |
|  5  |$$5^2 - 5 + 11$$| 31 |
|  6  |$$6^2 - 6 + 11$$| 41 |
|  7  |$$7^2 - 7 + 11$$| 53 |
|  8  |$$8^2 - 8 + 11$$| 67 |
|  9  |$$9^2 - 9 + 11$$| 83 |
|  10  |$$10^2 - 10 + 11$$| 101 |
19. a. Rewrite the following theorem in three different ways: as $\forall $ , if then, as $\forall$ (without using the words if or then), and as If , then  (without using an explicit universal quantiﬁer). 

    b. Fill in the blanks in the proof of the theorem.

    **Theorem:** The sum of any even integer and any odd integer is odd.

    **Proof:** Suppose m is any even integer and n is <u>(a)</u> . By deﬁnition of even, $m = 2r$ for some <u>(b)</u> , and by deﬁnition of odd, $n = 2s + 1$ for some integer $s$. By substitution and algebra,

    $$m + n = (c) = 2(r + s) + 1$$.

    Since r and s are both integers, so is their sum $r + s$. Hence $m + n$ has the form twice some integer plus one, and so <u>(d)</u> by deﬁnition of odd.

    **Answer**:

    a. 

    - $\forall$ integers m and n, if m is even and n is odd, then their sum $m+n$ is odd.

    - $\forall$ even integers m and odd integers n, their sum $m + n$ is odd.

    - If m is an even integer and n i an odd integer, their sum $m + n$ is odd.

    b.

    (a). any odd integer

    (b). integer r

    (c). $2r + 2s + 1$

    (d). $m + n$

20. For all integers m, if $m > 1$ then $0 < \frac{1}{m} < 1$.
    (a). If m is an integer and  $m > 1$, then $0 < \frac{1}{m} < 1$.

    (b).
        First sentence of the proof = Suppose that m is an integer greater than 1.
        Last sentence of the proof = $0 < \frac{1}{m} < 1$.

21. For all real numbers x, if x > 1 then $x^2 > x$.

    (a). If x is a real number and x > 1, then $x^2 > x$.

    (b).First sentence of the proof = Suppose that x is an real number greater than 1.
        Last sentence of the proof = $x^2 > x$.

22. For all integers m and n, if mn = 1 then m = n = 1 or m = n = −1.

    (a). If m and n are integers wiht $mn = 1$, then $m = n = 1 \or m = n = -1$.

    (b).First sentence of the proof = Suppose that m and n are integers such that $mn = 1$.
        Last sentence of the proof = $m = n = 1 \or m = n = -1$.

23. For all real numbers x, if 0 < x < 1 then $x^2 < x$.

    (a). If x is a positive real number and less than 1, then the square of it is smaller than itself.

    (b).First sentence of the proof = Suppose that x is a real number between 0 and 1.
        Last sentence of the proof = $x^2 < x$.

24. The negative of any even integer is even.

    Proof: Assum m is an even integer. Since $-m = 2\times(-k)$ can be written as twice some integer $-k$, $-m$ is even.

25. The difference of any even integer minus any odd integer is odd.

    Proof: Assume $m$ is an even integer and $n$ is an odd integer.
            $m - n = 2a - 2b - 1 = 2(a - b - 1) + 1$
            Since $a - b - 1$ is an integer, and $m - n$ can be written..., thus $m - n$ is odd.

26. The difference between any odd integer and any even integer is odd. (Note: The “proof” shown in exericse 39 contains an error. Can you spot it?)
    
    Proof: Assum $m$ is an odd integer and $n$ is an even integer.
            then we have: $m - n = 2a + 1 - 2b = 2(a - b) + 1$
            Since $(a - b)$ is an integer (the difference of two integers are integer) and ...

    'k' and 'k' are different.

27. The sum of any two odd integers is even.

    $$2(a + b + 1)$$

28. For all integers n, if n is odd then n^2 is odd.

    $$n^2 = (2a + 1)^2 = 2(2a^2 + 2a) + 1$$

29. For all integers n, if n is odd then 3n + 5 is even.

    $$2(3a + 4)$$

30. For all integers m, if m is even then 3m + 5 is odd.

    $$2(3a + 2) + 1$$

31. If k is any odd integer and m is any even integer, then, $k^2 + m^2$ is odd.

    $$2(2a^2 + 2a + 2b^2) + 1$$

32. If a is any odd integer and b is any even integer, then, 2a + 3b is even.
    
    $$2(2p + 1 + 3q)$$

33. If n is any even integer, then (−1)^n = 1.

    $$((-1)^{2})^k = 1$$

34. If n is any odd integer, then (−1)^n = −1.

   $$1^k \times (-1) = -1$$ 

35. There exists an integer m ≥ 3 such that m^2 − 1 is prime.   

    Assume is true then $m^2 - 1 = (m - 1)(m + 1)$. Since $m \geq 3$ ....

36. There exists an integer n such that $6n^2 + 27$ is prime.

    $$3(2n^2 + 9)$$, factor greater than 1 and smaller then itself.

37. There exists an integer k ≥ 4 such that $2k^2 − 5k + 2$ is prime.

    $$(2k - 1)(k - 2)$$
    
38. Theorem: For all integers k, if k > 0 then k 2 + 2k + 1 is composite. “Proof: For k = 2, k 2 + 2k + 1 = 2 2 + 2·2 + 1 = 9. But 9 = 3·3, and so 9 is composite. Hence the theorem is true.”

    Not for all integers.    

39. Theorem: The difference between any odd integer and any even integer is odd.
    “Proof: Suppose n is any odd integer, and m is any even integer. By deﬁnition of odd, n = 2k + 1 where k is an integer, and by deﬁnition of even, m = 2k where k is an integer. Then
    $$n - m = 2k + 1 - 2k = 1$$
    But 1 is odd. Therefore, the difference between any odd integer and any even integer is odd.”

    Not the same k.

40. Theorem: For all integers k, if k > 0 then $k^2+ 2k + 1$ is composite.
    “Proof: Suppose k is any integer such that k > 0. If $k^2 + 2k + 1$ is composite, then $k^2 + 2k + 1 = rs$ for some integers r and s such that
    $$1 < r < k^2 + 2k + 1$$ and
    $$1 < s < k^2 + 2k + 1$$
    Since $k^2 + 2k + 1 = rs$
    and both r and s are strictly between 1 and $k^2 + 2k + 1$, then $k^2 + 2k + 1$ is not prime. Hence $k^2 + 2k + 1$ is composite as was to be shown.”

    Circular reasoning.

41. Theorem: The product of an even integer and an odd integer is even.

    “Proof: Suppose m is an even integer and n is an odd integer. If $m·n$ is even, then by deﬁnition of even there exists an integer r such that $m·n = 2r$. Also since m is even, there exists an integer p such that $m = 2p$, and since n is odd there exists an integer q such that $n = 2q + 1$. Thus
    $$mn = (2p)(2q + 1) = 2r$$,
    where r is an integer. By definition of even, then, $m·n$ is even, as was to be shown.”

    Circular reasoning. We can't assume $m\cdot n$ is true when we want to prove it. 

42. Theorem: The sum of any two even integers equals 4k for some integer k.
    “Proof: Suppose m and n are any two even integers. By deﬁnition of even, m = 2k for some integer k and n = 2k for some integer k. By substitution,
    $$m + n = 2k + 2k = 4k$$.
    This is what was to be shown.”

    Implies m = n.

50. For all integers n and m, if n − m is even then $n^3 − m^3$ is even.
    
    $$ n^3 - m^3 = (n-m)(n^2 +nm + m^2) = 2(k(n^2 + nm + m^2))$$

53. For all integers n, $n^2 − n + 11$ is a prime number.

    $$11^2 - 11 + 11 = 121$$ is not a prime.

54. For all integers n, $4(n^2 + n + 1) − 3n^2$ is a perfect square.

    **perfect square**: iff $\exists k \in Z, n = k^2$

    $$n^2 + 4n + 4 = (n+2)^2$$. True

55. Every positive integer can be expressed as a sum of three or fewer perfect squares.

    False. 7 = 4 + 1 + 1 + 1 (only 1 or 4 can be used)

56. (Two integers are consecutive if, and only if, one is one more than the other.) Any product of four consecutive integers is one less than a perfect square.
    
    $$n(n+1)(n+2)(n+3) = (n^2 + n)(n^2 + 5n + 6) = (n^4 + 6n^3 + 11n^2 + 6n + 1) - 1 = (n^2 + 3n + 1)^2 - 1$$

    $$(x^2 + bx + c)^2 = x^4 + 2bx^3 + (b^2 + 2x)x^2 + 2bcx + x^2$$

    True.

57. If m and n are positive integers and mn is a perfect square, then m and n are perfect squares.

    $$3\times3 = 9$$. False.

58. The difference of the squares of any two consecutive integers is odd.
    
    $$(n+1)^2 - n^2 = 2n + 1$$. True.

59. For all nonnegative real numbers a and b, $\sqrt{ab} = \sqrt{a}\sqrt{b}$. (Note that if x is a nonnegative real number, then there is a unique nonnegative real number y, denoted $\sqrt{x}$, such that $y^2 = x$.

    There exists a real number p, q and r such that:
    $$p^2 = a$$
    $$q^2 = b$$
    $$r^2 = ab$$
